fix a few BigInts

lib/Buckets/PackedKV.i.dfy
@@ -1,10 +1,9 @@
 include "PackedStringArray.i.dfy"
 include "../Base/total_order.i.dfy"
-include "KVList.i.dfy"
+include "BucketsLib.i.dfy"
 
 module PackedKV {
-  import PackedStringArray
-  import KVList
+  import PSA = PackedStringArray
   import opened NativeTypes
   import Keyspace = Lexicographic_Byte_Order
   import opened KeyType
@@ -12,11 +11,16 @@ module PackedKV {
   import opened ValueMessage
   import opened BucketsLib
   import opened Options
-
+  import opened Sequences
+  import opened Maps
+  import Integer_Order
+  
   datatype Pkv = Pkv(
-      keys: PackedStringArray.Psa,
-      messages: PackedStringArray.Psa)
+      keys: PSA.Psa,
+      messages: PSA.Psa)
 
+  // TODO(robj): Ideally these constraints would be moved out of this
+  // "pure" data structure.
   predicate ValidKeyByteString(s: seq<byte>)
   {
     |s| <= KeyType.MaxLen() as int
@@ -27,38 +31,22 @@ module PackedKV {
     |s| <= ValueType.MaxLen() as int
   }
 
-  predicate ValidKeyLens(psa: PackedStringArray.Psa)
-  requires PackedStringArray.WF(psa)
+  predicate ValidStringLens<A>(strs: seq<seq<A>>, upper_bound: nat)
   {
-    forall i | 0 <= i < |psa.offsets| ::
-        PackedStringArray.psaEnd(psa, i as uint64) as int - PackedStringArray.psaStart(psa, i as uint64) as int <= KeyType.MaxLen() as int
+    forall i | 0 <= i < |strs| :: |strs[i]| <= upper_bound
   }
 
-  predicate WF(pkv: Pkv) {
-    && PackedStringArray.WF(pkv.keys)
-    && PackedStringArray.WF(pkv.messages)
-    && ValidKeyLens(pkv.keys)
-    && |pkv.keys.offsets| == |pkv.messages.offsets|
-  }
-
-  function {:opaque} psaSeq_Keys(psa: PackedStringArray.Psa, i: int) : (res : seq<Key>)
-  requires PackedStringArray.WF(psa)
-  requires ValidKeyLens(psa)
-  requires 0 <= i <= |psa.offsets|
-  ensures |res| == i
-  ensures forall j | 0 <= j < i :: res[j] == PackedStringArray.psaElement(psa, j as uint64)
+  predicate ValidKeyLens<A>(strs: seq<seq<A>>)
   {
-    if i == 0 then [] else psaSeq_Keys(psa, i-1) + [PackedStringArray.psaElement(psa, (i-1) as uint64)]
+    ValidStringLens(strs, KeyType.MaxLen() as nat)
   }
 
-  function IKeys(psa: PackedStringArray.Psa) : (res : seq<Key>)
-  requires PackedStringArray.WF(psa)
-  requires ValidKeyLens(psa)
+  predicate ValidMessageLens<A>(strs: seq<seq<A>>)
   {
-    psaSeq_Keys(psa, |psa.offsets|)
+    ValidStringLens(strs, ValueType.MaxLen() as nat)
   }
 
-  function method byteString_to_Message(s: seq<byte>) : Message
+  function method bytestring_to_Message(s: seq<byte>) : Message
   requires |s| < 0x1_0000_0000
   {
     if |s| as uint64 <= ValueType.MaxLen() then (
@@ -71,39 +59,50 @@ module PackedKV {
     )
   }
 
-  function {:opaque} psaSeq_Messages(psa: PackedStringArray.Psa, i: int) : (res : seq<Message>)
-  requires PackedStringArray.WF(psa)
-  requires 0 <= i <= |psa.offsets|
-  ensures |res| == i
-  ensures forall j | 0 <= j < i :: res[j] == byteString_to_Message(PackedStringArray.psaElement(psa, j as uint64))
+  function method Message_to_bytestring(msg: Message) : seq<byte>
+    requires msg.Define?
   {
-    if i == 0 then [] else psaSeq_Messages(psa, i-1) + [
-        byteString_to_Message(PackedStringArray.psaElement(psa, (i-1) as uint64))]
+    msg.value
+  }
+  
+  function IKeys(psa: PSA.Psa) : (res : seq<Key>)
+  requires PSA.WF(psa)
+  requires ValidStringLens(PSA.I(psa), KeyType.MaxLen() as nat)
+  {
+    PSA.I(psa)
   }
 
-  function IMessages(psa: PackedStringArray.Psa) : (res : seq<Message>)
-  requires PackedStringArray.WF(psa)
+  function {:opaque} psaSeq_Messages(psa: PSA.Psa, i: int) : (res : seq<Message>)
+  requires PSA.WF(psa)
+  requires 0 <= i <= |psa.offsets|
+  ensures |res| == i
+  ensures forall j | 0 <= j < i :: res[j] == bytestring_to_Message(PSA.psaElement(psa, j as uint64))
+  {
+    if i == 0 then [] else psaSeq_Messages(psa, i-1) + [
+        bytestring_to_Message(PSA.psaElement(psa, (i-1) as uint64))]
+  }
+
+  function IMessages(psa: PSA.Psa) : (res : seq<Message>)
+  requires PSA.WF(psa)
   {
     psaSeq_Messages(psa, |psa.offsets|)
   }
 
-  function IMapi(pkv: Pkv, i: int) : (bucket : BucketMap)
-  requires WF(pkv)
-  requires 0 <= i <= |pkv.keys.offsets|
-  ensures WFBucketMap(bucket)
-  {
-    if i == 0 then map[] else (
-      var key : Key := PackedStringArray.psaElement(pkv.keys, (i-1) as uint64);
-      var msg : Message := byteString_to_Message(PackedStringArray.psaElement(pkv.keys, (i-1) as uint64));
-      IMapi(pkv, i-1)[key := msg]
-    )
+  predicate WF(pkv: Pkv) {
+    && PSA.WF(pkv.keys)
+    && PSA.WF(pkv.messages)
+    && |pkv.keys.offsets| == |pkv.messages.offsets|
+    && ValidKeyLens(PSA.I(pkv.keys))
+    && ValidMessageLens(PSA.I(pkv.messages))
+    && IdentityMessage() !in IMessages(pkv.messages)
   }
 
   function IMap(pkv: Pkv) : (bucket : BucketMap)
   requires WF(pkv)
   ensures WFBucketMap(bucket)
   {
-    IMapi(pkv, |pkv.keys.offsets|)
+    assert IdentityMessage() !in Set(IMessages(pkv.messages));
+    BucketMapOfSeq(IKeys(pkv.keys), IMessages(pkv.messages))
   }
 
   predicate SortedKeys(pkv: Pkv)
@@ -117,62 +116,105 @@ module PackedKV {
   ensures WFBucket(bucket)
   {
     // Note that this might not be WellMarshalled
-    //reveal_WFBucket();
-    assume false;
     BucketMapWithSeq(IMap(pkv), IKeys(pkv.keys), IMessages(pkv.messages))
   }
 
-  method ComputeValidKeyLens(psa: PackedStringArray.Psa)
-  returns (b: bool)
-  requires PackedStringArray.WF(psa)
-  ensures b == ValidKeyLens(psa)
+  function method EmptyPkv() : (result: Pkv)
+    ensures WF(result)
+    ensures IMap(result) == map[]
   {
-    assume false; 
+    Pkv(PSA.EmptyPsa(), PSA.EmptyPsa())
+  }
 
-    if |psa.offsets| as uint64 == 0 {
-      return true;
-    }
-    if psa.offsets[0 as uint64] as uint64 > KeyType.MaxLen() {
-      return false;
-    }
+  function method NumKVPairs(pkv: Pkv) : uint64
+    requires WF(pkv)
+  {
+    PSA.psaNumStrings(pkv.keys)
+  }
+  
+  method ComputeValidStringLens(psa: PSA.Psa, upper_bound: uint64)
+  returns (b: bool)
+  requires PSA.WF(psa)
+  ensures b == ValidStringLens(PSA.I(psa), upper_bound as nat)
+  {
+    var i: uint64 := 0;
 
-    var i: uint64 := 1;
-    while i < |psa.offsets| as uint64
+    while i < PSA.psaNumStrings(psa)
+      invariant i <= PSA.psaNumStrings(psa)
+      invariant forall j | 0 <= j < i :: |PSA.I(psa)[j]| <= upper_bound as nat
     {
-      if psa.offsets[i] as uint64 - psa.offsets[i-1] as uint64 > KeyType.MaxLen() {
-        return false;
+      assert |PSA.I(psa)[i]| == PSA.psaEnd(psa, i) as nat - PSA.psaStart(psa, i) as nat;
+      if upper_bound < PSA.psaEnd(psa, i) as uint64 - PSA.psaStart(psa, i) as uint64 {
+        b := false;
+        return;
       }
       i := i + 1;
     }
+    
+    return true;
+  }
 
+  method ComputeIsSorted(pkv: Pkv)
+    returns (b: bool)
+    requires PSA.WF(pkv.keys)
+    ensures b == Keyspace.IsStrictlySorted(PSA.I(pkv.keys))
+  {
+    ghost var ikeys := PSA.I(pkv.keys);
+    
+    Keyspace.reveal_IsStrictlySorted();
+
+    if |pkv.keys.offsets| <= 1 {
+      return true;
+    }
+    
+    var i: uint64 := 0;
+    while i < |pkv.keys.offsets| as uint64 - 1
+      invariant i as int <= |pkv.keys.offsets| - 1
+      invariant Keyspace.IsStrictlySorted(ikeys[..i+1])
+    {
+      var c := Keyspace.cmp(PSA.psaElement(pkv.keys, i), PSA.psaElement(pkv.keys, i+1));
+      if c >= 0 {
+        assert PSA.I(pkv.keys)[i] == PSA.psaElement(pkv.keys, i);
+        assert PSA.I(pkv.keys)[i+1] == PSA.psaElement(pkv.keys, i+1);
+        return false;
+      }
+      Keyspace.StrictlySortedAugment(ikeys[..i+1], ikeys[i+1]);
+      assert ikeys[..i+2] == ikeys[..i+1] + [ikeys[i+1]];
+      i := i + 1;
+    }
+    
+    assert ikeys == ikeys[..i+1];
+      
     return true;
   }
 
   function SizeOfPkv(pkv: Pkv) : int
   {
-    PackedStringArray.SizeOfPsa(pkv.keys) + PackedStringArray.SizeOfPsa(pkv.messages)
+    PSA.SizeOfPsa(pkv.keys) + PSA.SizeOfPsa(pkv.messages)
   }
 
   function method SizeOfPkvUint64(pkv: Pkv) : uint64
   requires WF(pkv)
   {
-    PackedStringArray.SizeOfPsaUint64(pkv.keys) + PackedStringArray.SizeOfPsaUint64(pkv.messages)
+    PSA.SizeOfPsaUint64(pkv.keys) + PSA.SizeOfPsaUint64(pkv.messages)
   }
 
   function method WeightPkv(pkv: Pkv) : uint64
   requires WF(pkv)
   {
-    4 * |pkv.keys.offsets| as uint64 + |pkv.keys.data| as uint64 +
-    4 * |pkv.messages.offsets| as uint64 + |pkv.messages.data| as uint64
+    4 + 4 * |pkv.keys.offsets| as uint64 + |pkv.keys.data| as uint64 +
+    4 + 4 * |pkv.messages.offsets| as uint64 + |pkv.messages.data| as uint64
   }
 
+  // I don't think we need these if we use the generic marshaling code. -- rob
+  
   function parse_Pkv(data: seq<byte>) : (res : (Option<Pkv>, seq<byte>))
   ensures res.0.Some? ==> WF(res.0.value)
   {
-    var (keys, rest1) := PackedStringArray.parse_Psa(data);
+    var (keys, rest1) := PSA.parse_Psa(data);
     if keys.Some? then (
-      if ValidKeyLens(keys.value) then (
-        var (messages, rest2) := PackedStringArray.parse_Psa(rest1);
+      if ValidKeyLens(PSA.I(keys.value)) then (
+        var (messages, rest2) := PSA.parse_Psa(rest1);
         if messages.Some?
             && |keys.value.offsets| == |messages.value.offsets| then (
           var res := Pkv(keys.value, messages.value);
@@ -197,13 +239,13 @@ module PackedKV {
       && pkv == pkv'
       && data[rest_index..] == rest'
   {
-    var keys, rest1 := PackedStringArray.Parse_Psa(data, index);
+    var keys, rest1 := PSA.Parse_Psa(data, index);
     if keys.Some? {
       // TODO we iterate twice, once to check sortedness, another
       // to check lengths, we could consolidate.
-      var isValidKeyLens := ComputeValidKeyLens(keys.value);
+      var isValidKeyLens := ComputeValidStringLens(keys.value, KeyType.MaxLen());
       if isValidKeyLens {
-        var messages, rest2 := PackedStringArray.Parse_Psa(data, rest1);
+        var messages, rest2 := PSA.Parse_Psa(data, rest1);
         if messages.Some?
             && |keys.value.offsets| as uint64 == |messages.value.offsets| as uint64 {
           pkv := Some(Pkv(keys.value, messages.value));
@@ -226,28 +268,39 @@ module PackedKV {
   requires WF(pkv)
   requires |pkv.keys.offsets| > 0
   {
-    PackedStringArray.FirstElement(pkv.keys)
+    assert PSA.FirstElement(pkv.keys) == PSA.I(pkv.keys)[0];
+    PSA.FirstElement(pkv.keys)
   }
 
   function method LastKey(pkv: Pkv) : Key
   requires WF(pkv)
   requires |pkv.keys.offsets| > 0
   {
-    PackedStringArray.LastElement(pkv.keys)
+    assert PSA.LastElement(pkv.keys) == Last(PSA.I(pkv.keys));
+    PSA.LastElement(pkv.keys)
   }
 
   function method GetKey(pkv: Pkv, i: uint64) : Key
   requires WF(pkv)
   requires 0 <= i as int < |pkv.keys.offsets|
   {
-    PackedStringArray.psaElement(pkv.keys, i)
+    assert PSA.psaElement(pkv.keys, i) == PSA.I(pkv.keys)[i];
+    PSA.psaElement(pkv.keys, i)
   }
 
   function method GetMessage(pkv: Pkv, i: uint64) : Message
   requires WF(pkv)
   requires 0 <= i as int < |pkv.messages.offsets|
   {
-    byteString_to_Message(PackedStringArray.psaElement(pkv.messages, i))
+    bytestring_to_Message(PSA.psaElement(pkv.messages, i))
+  }
+
+  function binarySearchPostProc(lo: nat, sub: Option<nat>) : Option<nat>
+  {
+    if sub.Some? then
+      Some(lo + sub.value)
+    else
+      None
   }
 
   method BinarySearchQuery(pkv: Pkv, key: Key)
@@ -255,12 +308,16 @@ module PackedKV {
   requires WF(pkv)
   ensures msg == bucketBinarySearchLookup(I(pkv), key)
   {
-    assume false;
-
+    ghost var keys := I(pkv).keys;
+    
     var lo: uint64 := 0;
     var hi: uint64 := |pkv.keys.offsets| as uint64;
 
+    assert keys == keys[lo..hi];
+    
     while lo < hi
+      invariant lo <= hi <= |pkv.keys.offsets| as uint64
+      invariant binarySearch(keys, key) == binarySearchPostProc(lo as nat, binarySearch(keys[lo..hi], key))
     {
       var mid: uint64 := (lo + hi) / 2;
       var c := Keyspace.cmp(key, GetKey(pkv, mid));
@@ -268,7 +325,10 @@ module PackedKV {
         msg := Some(GetMessage(pkv, mid));
         return;
       } else if (c < 0) {
+        ghost var rkeys := keys[lo..hi];
+        ghost var rmid := |rkeys| / 2;
         hi := mid;
+        assert keys[lo..hi] == rkeys[..rmid];
       } else {
         lo := mid + 1;
       }
@@ -277,21 +337,722 @@ module PackedKV {
     msg := None;
   }
 
-  method ComputeIsSorted(pkv: Pkv)
-    returns (b: bool)
-    requires PackedStringArray.WF(pkv.keys)
-    ensures b == Keyspace.IsStrictlySorted(PackedStringArray.I(pkv.keys))
+  predicate canAppend(pkv: Pkv, key: Key, msg: seq<byte>)
+    requires WF(pkv)
   {
-    assume false;
-    var i: uint64 := 1;
-    while i < |pkv.keys.offsets| as uint64
+    && PSA.psaCanAppend(pkv.keys, key)
+    && PSA.psaCanAppend(pkv.messages, msg)
+    && ValidMessageByteString(msg)
+  }
+
+  function AppendEncodedMessage(pkv: Pkv, key: Key, msg: seq<byte>) : (result: Pkv)
+    requires WF(pkv)
+    requires canAppend(pkv, key, msg)
+    ensures WF(result)
+  {
+    PSA.psaAppendIAppend(pkv.keys, key);
+    PSA.psaAppendIAppend(pkv.messages, msg);
+    Pkv(PSA.psaAppend(pkv.keys, key), PSA.psaAppend(pkv.messages, msg))
+  }
+  
+  function Append(pkv: Pkv, key: Key, msg: Message) : (result: Pkv)
+    requires WF(pkv)
+    requires msg.Define?
+    requires canAppend(pkv, key, Message_to_bytestring(msg))
+    ensures WF(result)
+  {
+    AppendEncodedMessage(pkv, key, Message_to_bytestring(msg))
+  }
+
+  lemma IMapAppend(pkv: Pkv, key: Key, msg: seq<byte>)
+    requires WF(pkv)
+    requires canAppend(pkv, key, msg)
+    ensures IMap(AppendEncodedMessage(pkv, key, msg)) == IMap(pkv)[key := bytestring_to_Message(msg)]
+  {
+    PSA.psaAppendIAppend(pkv.keys, key);
+    PSA.psaAppendIAppend(pkv.messages, msg);
+    var keys := PSA.I(pkv.keys);
+    var messages := IMessages(pkv.messages);
+    var newpkv := AppendEncodedMessage(pkv, key, msg);
+    var newkeys := PSA.I(newpkv.keys);
+    var newmessages := IMessages(newpkv.messages);
+
+    assert forall i | 0 <= i < |messages| :: Sequences.DropLast(newmessages)[i] == bytestring_to_Message(PSA.I(newpkv.messages)[i]);
+    assert Sequences.DropLast(newmessages) == messages;
+    assert Last(newmessages) == bytestring_to_Message(msg);
+
+    calc {
+      IMap(newpkv);
+      { reveal_BucketMapOfSeq(); }
+      BucketMapOfSeq(keys, messages)[key := bytestring_to_Message(msg)];
+      { reveal_BucketMapOfSeq(); }
+      IMap(pkv)[key := bytestring_to_Message(msg)];
+    }
+  }
+
+  function subPkv(pkv: Pkv, from: uint64, to: uint64) : (result: Pkv)
+    requires WF(pkv)
+    requires 0 <= from <= to <= PSA.psaNumStrings(pkv.keys)
+    ensures WF(result)
+  {
+    Pkv(PSA.psaSubSeq(pkv.keys, from, to), PSA.psaSubSeq(pkv.messages, from, to))
+  }
+
+  method SubPkv(pkv: Pkv, from: uint64, to: uint64) returns (result: Pkv)
+    requires WF(pkv)
+    requires 0 <= from <= to <= PSA.psaNumStrings(pkv.keys)
+    ensures result == subPkv(pkv, from, to)
+  {
+    var subkeys := PSA.PsaSubSeq(pkv.keys, from, to);
+    var submessages := PSA.PsaSubSeq(pkv.messages, from, to);
+    result := Pkv(subkeys, submessages);
+  }
+  
+  function DropLast(pkv: Pkv) : (result: Pkv)
+    requires WF(pkv)
+    requires 0 < NumKVPairs(pkv)
+    ensures WF(result)
+  {
+    subPkv(pkv, 0, NumKVPairs(pkv) - 1)
+  }
+
+  lemma Imaps(pkv: Pkv, i: int)
+    requires WF(pkv)
+    requires Keyspace.IsStrictlySorted(PSA.I(pkv.keys))
+    requires 0 <= i < |PSA.I(pkv.keys)|
+    ensures MapsTo(IMap(pkv), PSA.I(pkv.keys)[i], bytestring_to_Message(PSA.I(pkv.messages)[i]))
+    decreases |PSA.I(pkv.keys)|
+  {
+    var ikeys := PSA.I(pkv.keys);
+    var imessages := PSA.I(pkv.messages);
+    
+    if (i == |ikeys| - 1) {
+      reveal_BucketMapOfSeq();
+    } else {
+      Keyspace.reveal_IsStrictlySorted();
+      reveal_BucketMapOfSeq();
+      Imaps(DropLast(pkv), i);
+      forall j | 0 <= j < |Sequences.DropLast(IMessages(pkv.messages))|
+        ensures Sequences.DropLast(IMessages(pkv.messages))[j] == IMessages(PSA.psaDropLast(pkv.messages))[j]
+      {
+        calc {
+          Sequences.DropLast(IMessages(pkv.messages))[j];
+          bytestring_to_Message(PSA.I(pkv.messages)[j]);
+        }
+      }
+      assert Sequences.DropLast(IMessages(pkv.messages)) == IMessages(PSA.psaDropLast(pkv.messages));
+    }
+  }
+
+  method SplitLeft(pkv: Pkv, pivot: Key) returns (result: Pkv)
+    requires WF(pkv)
+    requires Keyspace.IsStrictlySorted(PSA.I(pkv.keys))
+    ensures WF(result)
+    ensures Keyspace.IsStrictlySorted(PSA.I(result.keys))
+    ensures I(result) == SplitBucketLeft(I(pkv), pivot)
+  {
+    var idx := PSA.IndexOfFirstKeyGte(pkv.keys, pivot);
+    result := SubPkv(pkv, 0, idx);
+
+    ghost var ikeys := PSA.I(pkv.keys);
+    ghost var subkeys := PSA.I(result.keys);
+    
+    Keyspace.StrictlySortedSubsequence(ikeys, 0, idx as int);
+    
+    ghost var a := IMap(result);
+    ghost var b := SplitBucketLeft(I(pkv), pivot).b;
+
+    forall key | key in a
+      ensures MapsTo(b, key, a[key])
     {
-      var c := Keyspace.cmp(GetKey(pkv, i-1), GetKey(pkv, i));
-      if c >= 0 {
-        return false;
+      var i := Sequences.IndexOf(ikeys, key);
+      Imaps(pkv, i);
+      Imaps(result, i);
+      reveal_SplitBucketLeft();
+    }
+
+    forall key | key in b
+      ensures key in a
+    {
+      reveal_SplitBucketLeft();
+    }
+
+    ghost var iresult := I(result);
+    ghost var isplit := SplitBucketLeft(I(pkv), pivot);
+    WellMarshalledBucketsEq(iresult, isplit);
+  }
+    
+  method SplitRight(pkv: Pkv, pivot: Key) returns (result: Pkv)
+    requires WF(pkv)
+    requires Keyspace.IsStrictlySorted(PSA.I(pkv.keys))
+    ensures WF(result)
+    ensures Keyspace.IsStrictlySorted(PSA.I(result.keys))
+    ensures I(result) == SplitBucketRight(I(pkv), pivot)
+  {
+    var idx := PSA.IndexOfFirstKeyGte(pkv.keys, pivot);
+    result := SubPkv(pkv, idx, NumKVPairs(pkv));
+
+    ghost var ikeys := PSA.I(pkv.keys);
+    ghost var subkeys := PSA.I(result.keys);
+    
+    Keyspace.StrictlySortedSubsequence(ikeys, idx as int, |ikeys|);
+    
+    ghost var a := IMap(result);
+    ghost var b := SplitBucketRight(I(pkv), pivot).b;
+
+    forall key | key in a
+      ensures MapsTo(b, key, a[key])
+    {
+      var i := Sequences.IndexOf(ikeys, key);
+      Imaps(pkv, i);
+      Imaps(result, i - idx as int);
+      reveal_SplitBucketRight();
+    }
+
+    forall key | key in b
+      ensures key in a
+    {
+      reveal_SplitBucketRight();
+    }
+
+    ghost var iresult := I(result);
+    ghost var isplit := SplitBucketRight(I(pkv), pivot);
+    WellMarshalledBucketsEq(iresult, isplit);
+  }
+
+  // TODO: add support for partial merges.  (slack is unused at the moment)
+  function mergeToOneChild(top: Pkv, from: nat, to: nat, bot: Pkv, slack: uint64) : (result: Option<Pkv>)
+    requires WF(top)
+    requires WF(bot)
+    requires from <= to <= NumKVPairs(top) as nat
+    ensures result.Some? ==> WF(result.value)
+    decreases to - from + NumKVPairs(bot) as nat
+  {
+    //assert 0 < NumKVPairs(top) ==> PSA.LastElement(top.keys) == Last(PSA.I(top.keys));
+    //assert 0 < NumKVPairs(bot) ==> PSA.LastElement(bot.keys) == Last(PSA.I(bot.keys));
+    if from == to then
+      Some(bot)
+    else if NumKVPairs(bot) == 0 then
+      Some(subPkv(top, from as uint64, to as uint64))
+    else if PSA.psaElement(top.keys, to as uint64 - 1) == PSA.LastElement(bot.keys) then (
+      var submerge := mergeToOneChild(DropLast(top), from, to-1, DropLast(bot), slack);
+      var key := PSA.psaElement(top.keys, to as uint64 - 1);
+      assert key == PSA.I(top.keys)[to-1];
+      var topmsg := bytestring_to_Message(PSA.psaElement(top.messages, to as uint64 - 1));
+      var botmsg := bytestring_to_Message(PSA.LastElement(bot.messages));
+      var msg := ValueMessage.Merge(topmsg, botmsg);
+      var bytemsg := Message_to_bytestring(msg);
+      if submerge == None || msg == IdentityMessage() then
+        submerge
+      else if !canAppend(submerge.value, key, bytemsg) then
+        None
+      else 
+        Some(AppendEncodedMessage(submerge.value, key, bytemsg))
+    ) else if Keyspace.lt(PSA.I(top.keys)[to - 1], Last(PSA.I(bot.keys))) then (
+      var submerge := mergeToOneChild(top, from, to, DropLast(bot), slack);
+      var key := PSA.LastElement(bot.keys);
+      assert key == PSA.I(bot.keys)[PSA.psaNumStrings(bot.keys)-1];
+      var msg := PSA.LastElement(bot.messages);
+      if submerge == None || !canAppend(submerge.value, key, msg) then
+        None
+      else 
+        Some(AppendEncodedMessage(submerge.value, key, msg))
+    ) else (
+      var submerge := mergeToOneChild(top, from, to-1, bot, slack);
+      var key := PSA.psaElement(top.keys, to as uint64 - 1);
+      assert key == PSA.I(top.keys)[to-1];
+      var msg := PSA.LastElement(top.messages);
+      if submerge == None || !canAppend(submerge.value, key, msg) then
+        None
+      else 
+        Some(AppendEncodedMessage(submerge.value, key, msg))
+    )    
+  }
+
+  lemma psaTotalLengthBound(psa: PSA.Psa, maxlen: nat)
+    requires PSA.WF(psa)
+    requires forall i | 0 <= i < |PSA.I(psa)| :: |PSA.I(psa)[i]| <= maxlen
+    ensures PSA.psaTotalLength(psa) as nat <= PSA.psaNumStrings(psa) as nat * maxlen
+    decreases PSA.psaNumStrings(psa)
+  {
+    var ipsa := PSA.I(psa);
+    if |ipsa| == 0 {
+    } else {
+      var prepsa := PSA.psaDropLast(psa);
+      psaTotalLengthBound(prepsa, maxlen);
+      PSA.psaAppendTotalLength(prepsa, Last(ipsa));
+    }
+  }
+  
+  // lemma MergeWillSucceed(top: Pkv, bot: Pkv) returns (result: Pkv)
+  //   requires WF(top)
+  //   requires WF(bot)
+  //   requires NumKVPairs(top) + NumKVPairs(bot) < 0x1_0000_0000
+  //   requires PSA.psaTotalLength(top.keys) + PSA.psaTotalLength(bot.keys) < 0x1_0000_0000
+  //   requires (NumKVPairs(top) as nat + NumKVPairs(bot) as nat) * (1 + ValueType.MaxLen() as nat) < 0x1_0000_0000
+  //   ensures Merge(top, bot) == Some(result)
+  //   ensures NumKVPairs(result) <= NumKVPairs(top) + NumKVPairs(bot)
+  //   ensures PSA.psaTotalLength(result.keys) <= PSA.psaTotalLength(top.keys) + PSA.psaTotalLength(bot.keys)
+  //   ensures PSA.psaTotalLength(result.messages) as nat
+  //   <= (NumKVPairs(top) as nat + NumKVPairs(bot) as nat) * (1 + ValueType.MaxLen() as nat)
+  //   decreases NumKVPairs(top) + NumKVPairs(bot)
+  // {
+  //   assert 0 < NumKVPairs(top) ==> PSA.LastElement(top.keys) == Last(PSA.I(top.keys));
+  //   assert 0 < NumKVPairs(bot) ==> PSA.LastElement(bot.keys) == Last(PSA.I(bot.keys));
+  //   if NumKVPairs(top) == 0 {
+  //     psaTotalLengthBound(bot.messages, ValueType.MaxLen() as nat);
+  //     result := bot;
+  //   } else if NumKVPairs(bot) == 0 {
+  //     psaTotalLengthBound(top.messages, ValueType.MaxLen() as nat);
+  //     result := top;
+  //   } else if PSA.LastElement(top.keys) == PSA.LastElement(bot.keys) {
+  //     var submerge := Merge(DropLast(top), DropLast(bot));
+  //     var key := PSA.LastElement(top.keys);
+  //     var topmsg := bytestring_to_Message(PSA.LastElement(top.messages));
+  //     var botmsg := bytestring_to_Message(PSA.LastElement(bot.messages));
+  //     var msg := ValueMessage.Merge(topmsg, botmsg);
+  //     var bytemsg := Message_to_bytestring(msg);
+  //     var submergepsa := MergeWillSucceed(DropLast(top), DropLast(bot));
+  //     if msg == IdentityMessage() {
+  //       result := submergepsa;
+  //     } else {
+  //       result := AppendEncodedMessage(submerge.value, key, bytemsg);
+  //     }
+  //   } else if Keyspace.lt(PSA.LastElement(top.keys), PSA.LastElement(bot.keys)) {
+  //     var submerge := Merge(top, DropLast(bot));
+  //     var key := PSA.LastElement(bot.keys);
+  //     var msg := PSA.LastElement(bot.messages);
+  //     assert msg == Last(PSA.I(bot.messages));
+  //     var submergepsa := MergeWillSucceed(top, DropLast(bot));
+  //     result := AppendEncodedMessage(submerge.value, key, msg);
+  //   } else {
+  //     var submerge := Merge(DropLast(top), bot);
+  //     var key := PSA.LastElement(top.keys);
+  //     var msg := PSA.LastElement(top.messages);
+  //     assert msg == Last(PSA.I(top.messages));
+  //     var submergepsa := MergeWillSucceed(DropLast(top), bot);
+  //     result := AppendEncodedMessage(submerge.value, key, msg);
+  //   }
+  // }
+
+  // lemma MergeWillSucceedNoReturn(top: Pkv, bot: Pkv)
+  //   requires WF(top)
+  //   requires WF(bot)
+  //   requires NumKVPairs(top) + NumKVPairs(bot) < 0x1_0000_0000
+  //   requires PSA.psaTotalLength(top.keys) + PSA.psaTotalLength(bot.keys) < 0x1_0000_0000
+  //   requires (NumKVPairs(top) as nat + NumKVPairs(bot) as nat) * (1 + ValueType.MaxLen() as nat) < 0x1_0000_0000
+  //   ensures Merge(top, bot).Some?
+  //   ensures NumKVPairs(Merge(top, bot).value) <= NumKVPairs(top) + NumKVPairs(bot)
+  //   ensures PSA.psaTotalLength(Merge(top, bot).value.keys)
+  //   <= PSA.psaTotalLength(top.keys) + PSA.psaTotalLength(bot.keys)
+  //   ensures PSA.psaTotalLength(Merge(top, bot).value.messages) as nat
+  //   <= (NumKVPairs(top) as nat + NumKVPairs(bot) as nat) * (1 + ValueType.MaxLen() as nat)
+  // {
+  //   var dummy := MergeWillSucceed(top, bot);
+  // }
+
+  function pivotIndexes(keys: seq<Key>, pivots: seq<Key>) : (result: seq<nat>)
+    requires Keyspace.IsStrictlySorted(keys)
+    ensures |result| == |pivots|
+    ensures forall i | 0 <= i < |result| :: result[i] == Keyspace.IndexOfFirstGte(keys, pivots[i])
+  {
+    if |pivots| == 0 then
+      []
+    else
+      pivotIndexes(keys, Sequences.DropLast(pivots)) + [ Keyspace.IndexOfFirstGte(keys, Last(pivots)) ]
+  }
+  
+  // function mergeToChildren(top: Pkv, pivots: seq<Key>, bots: seq<Pkv>, slack: nat) : (result: seq<Option<Pkv>>)
+  //   requires WF(top)
+  //   requires Integer_Order.IsSorted(pivotIdxs)
+  //   requires 0 < |bots| == |pivotIdxs|
+  //   requires Last(pivotIdxs) <= NumKVPairs(top) as nat
+  //   requires forall i | 0 <= i < |bots| :: WF(bots[i])
+  // {
+  //   // if |pivotIdxs| == 1 then
+  //   //   [ mergeToOneChild(top, 0, pivotIdxs[0], bots[0]) ]
+  //   // else
+  //   //   Integer_Order.SortedSubsequence(pivotIdxs, 0, |pivotIdxs| - 1);
+  //   //   Integer_Order.IsSortedImpliesLte(pivotIdxs, |pivotIdxs| - 2, |pivotIdxs| - 1);
+  //   //   var submerge := mergeToChildren(top, Sequences.DropLast(pivotIdxs), Sequences.DropLast(bots));
+  //   //   var lastmerge := mergeToOneChild(top, pivotIdxs[|pivotIdxs|-2], Last(pivotIdxs), Last(bots));
+  //   //   submerge + [ lastmerge ]
+  // }
+
+}
+
+module DynamicPkv {
+  import PKV = PackedKV
+  import PSA = PackedStringArray
+  import opened KeyType
+  import opened ValueType`Internal
+  import opened ValueMessage
+  import opened NativeTypes
+  import Seq = Sequences
+  import Uint64_Order
+  import LexOrder = Lexicographic_Byte_Order
+  import opened BucketsLib
+  
+  datatype Capacity = Capacity(num_kv_pairs: uint32, total_key_len: uint32, total_message_len: uint32)
+
+  function method EmptyCapacity() : Capacity
+  {
+    Capacity(0, 0, 0)
+  }
+    
+  class DynamicPkv {
+    var keys: PKV.PSA.DynamicPsa
+    var messages: PKV.PSA.DynamicPsa
+    ghost var Repr: set<object>
+
+    predicate WF()
+      reads this, this.Repr
+    {
+      && this in Repr
+      && keys in Repr
+      && keys.Repr <= Repr
+      && messages in Repr
+      && messages.Repr <= Repr
+      && {this} !! keys.Repr !! messages.Repr 
+      && keys.WF()
+      && messages.WF()
+      && PKV.WF(PKV.Pkv(keys.toPsa(), messages.toPsa()))
+    }
+
+    function method toPkv() : PKV.Pkv
+      requires WF()
+      reads this, this.Repr
+    {
+      PKV.Pkv(keys.toPsa(), messages.toPsa())
+    }
+
+    function method weight() : uint64
+      requires WF()
+      reads this, this.Repr
+    {
+      keys.weight() + messages.weight()
+    }
+    
+    method AppendEncodedMessage(key: Key, msg: seq<byte>)
+      requires WF()
+      requires PKV.canAppend(toPkv(), key, msg)
+      ensures WF()
+      ensures toPkv() == PKV.AppendEncodedMessage(old(toPkv()), key, msg)
+      ensures fresh(Repr - old(Repr))
+      modifies this, Repr
+    {
+      keys.Append(key);
+      messages.Append(msg);
+      Repr := {this} + keys.Repr + messages.Repr;
+      assert PKV.Pkv(keys.toPsa(), messages.toPsa()) == PKV.AppendEncodedMessage(old(toPkv()), key, msg);
+    }
+    
+    method Append(key: Key, msg: Message)
+      requires WF()
+      requires msg.Define?
+      requires PKV.canAppend(toPkv(), key, PKV.Message_to_bytestring(msg))
+      ensures WF()
+      ensures toPkv() == PKV.Append(old(toPkv()), key, msg)
+      ensures fresh(Repr - old(Repr))
+      modifies this, Repr
+    {
+      AppendEncodedMessage(key, PKV.Message_to_bytestring(msg));
+    }
+
+    predicate hasCapacity(cap: Capacity)
+      requires WF()
+      reads Repr
+    {
+      && cap.num_kv_pairs as int <= keys.offsets.Length
+      && cap.total_key_len as int <= keys.data.Length
+      && cap.num_kv_pairs as int <= messages.offsets.Length
+      && cap.total_message_len as int <= messages.data.Length
+    }
+
+    constructor PreSized(capacity: Capacity)
+      ensures WF()
+      ensures hasCapacity(capacity)
+      ensures toPkv() == PKV.EmptyPkv()
+      ensures fresh(Repr)
+    {
+      keys := new PKV.PSA.DynamicPsa.PreSized(capacity.num_kv_pairs, capacity.total_key_len);
+      messages := new PKV.PSA.DynamicPsa.PreSized(capacity.num_kv_pairs, capacity.total_message_len);
+      new;
+      Repr := {this} + keys.Repr + messages.Repr;
+    }
+  }
+
+  
+  
+  datatype SingleMergeResult =
+      MergeCompleted(bot: PKV.Pkv, slack: uint64)
+    | SlackExhausted(bot: PKV.Pkv, end: uint64, slack: uint64)
+  
+  predicate MergeIsCorrectIfInputsWereSorted(top: PKV.Pkv, from: uint64, to: uint64,
+    bot: PKV.Pkv, result: SingleMergeResult)
+    requires PKV.WF(top)
+    requires PKV.WF(bot)
+    requires to as nat - from as nat + PKV.NumKVPairs(bot) as nat < Uint32UpperBound()
+    requires from <= to <= PKV.NumKVPairs(top)
+    requires PKV.WF(result.bot)
+    requires result.SlackExhausted? ==> from <= result.end < to
+  {
+    if
+      && BucketWellMarshalled(PKV.I(top))
+      && BucketWellMarshalled(PKV.I(bot))
+    then (
+      var subtop := PKV.subPkv(top, from, to);
+      var oldcomp := Compose(PKV.I(subtop), PKV.I(bot));
+      var newcomp :=
+        if result.MergeCompleted? then
+          PKV.I(result.bot)
+        else (
+          var newsubtop := PKV.subPkv(top, result.end, to);
+          Compose(PKV.I(newsubtop), PKV.I(result.bot))
+        );
+      && BucketWellMarshalled(PKV.I(result.bot))
+      && BucketsEquivalent(oldcomp, newcomp)
+    ) else
+      true
+  }
+
+  method MergeToOneChild(top: PKV.Pkv, from: uint64, to: uint64, bot: PKV.Pkv, slack: uint64)
+    returns (result: SingleMergeResult)
+    requires PKV.WF(top)
+    requires PKV.WF(bot)
+    requires PKV.Keyspace.IsStrictlySorted(PSA.I(top.keys))
+    requires PKV.Keyspace.IsStrictlySorted(PSA.I(bot.keys))
+    requires to as nat - from as nat + PKV.NumKVPairs(bot) as nat < Uint32UpperBound()
+    requires PKV.WeightPkv(bot) as nat + slack as nat < Uint32UpperBound()
+    requires from <= to <= PKV.NumKVPairs(top)
+    ensures PKV.WF(result.bot)
+    ensures result.slack <= PKV.WeightPkv(bot) + slack
+    ensures PKV.WeightPkv(result.bot) <= PKV.WeightPkv(bot) + slack - result.slack
+    ensures result.SlackExhausted? ==> from <= result.end < to
+  {
+    var maxkeys: uint32 := (to - from + PKV.NumKVPairs(bot)) as uint32;
+    var maxkeyspace: uint32 := (PSA.psaTotalLength(bot.keys) + slack) as uint32;
+    var maxmsgspace: uint32 := (PSA.psaTotalLength(bot.messages) + slack) as uint32;
+    var cap := Capacity(maxkeys, maxkeyspace, maxmsgspace);
+    var dresult := new DynamicPkv.PreSized(cap);
+
+    var runningSlack := slack;
+    var topidx: uint64 := from;
+    var botidx: uint64 := 0;
+
+    assert PKV.Keyspace.IsStrictlySorted(PSA.I(dresult.keys.toPsa())) by {
+      PKV.Keyspace.reveal_IsStrictlySorted();
+    }
+    
+    while
+      && topidx < to
+      && botidx < PKV.NumKVPairs(bot)
+      invariant from <= topidx <= to
+      invariant botidx <= PKV.NumKVPairs(bot)
+      invariant dresult.keys.nstrings <= botidx + topidx - from
+      invariant runningSlack <= slack
+      invariant dresult.WF()
+      invariant dresult.weight() <= PKV.WeightPkv(PKV.subPkv(bot, 0, botidx)) + slack - runningSlack
+      invariant fresh(dresult.Repr)
+      invariant 0 < |PSA.I(dresult.keys.toPsa())| && topidx < to ==>
+        PKV.Keyspace.lt(Seq.Last(PSA.I(dresult.keys.toPsa())), PSA.I(top.keys)[topidx])
+      invariant 0 < |PSA.I(dresult.keys.toPsa())| && botidx as nat < |PSA.I(bot.keys)| ==>
+        PKV.Keyspace.lt(Seq.Last(PSA.I(dresult.keys.toPsa())), PSA.I(bot.keys)[botidx])
+      invariant PKV.Keyspace.IsStrictlySorted(PSA.I(dresult.keys.toPsa()))
+      decreases to - topidx + PSA.psaNumStrings(bot.keys) - botidx
+    {
+      var topkey := PKV.GetKey(top, topidx);
+      var botkey := PKV.GetKey(bot, botidx);
+      var topmsg := PSA.psaElement(top.messages, topidx);
+      var botmsg := PSA.psaElement(bot.messages, botidx);
+      assert botmsg == PSA.I(bot.messages)[botidx];
+      assert topmsg == PSA.I(top.messages)[topidx];
+      
+      if botidx as nat + 1 < |PSA.I(bot.keys)| {
+        PKV.Keyspace.IsStrictlySortedImpliesLt(PSA.I(bot.keys), botidx as nat, botidx as nat + 1);
+      }
+      if topidx + 1 < to {
+        PKV.Keyspace.IsStrictlySortedImpliesLt(PSA.I(top.keys), topidx as nat, topidx as nat + 1);
+      }
+      PSA.psaAppendIAppend(dresult.keys.toPsa(), PSA.I(bot.keys)[botidx]);
+      PKV.Keyspace.StrictlySortedAugment(PSA.I(dresult.keys.toPsa()), PSA.I(bot.keys)[botidx]);
+      if PSA.psaCanAppend(dresult.keys.toPsa(), PSA.I(top.keys)[topidx]) {
+        PSA.psaAppendIAppend(dresult.keys.toPsa(), PSA.I(top.keys)[topidx]);
+        PKV.Keyspace.StrictlySortedAugment(PSA.I(dresult.keys.toPsa()), PSA.I(top.keys)[topidx]);
+      }
+
+      var c := PKV.Keyspace.cmp(botkey, topkey);
+
+      if c < 0 {
+        var botmsg := PSA.psaElement(bot.messages, botidx);
+        dresult.AppendEncodedMessage(botkey, botmsg);
+        // no change is slack
+        botidx := botidx + 1;
+      } else if c > 0 {
+        var topmsg := PSA.psaElement(top.messages, topidx);
+        var kvweight := 4 + |topkey| as uint64 + 4 + |topmsg| as uint64;
+        if kvweight < runningSlack {
+          dresult.AppendEncodedMessage(topkey, topmsg);
+          runningSlack := runningSlack - kvweight;
+          topidx := topidx + 1;
+        } else {
+          break;
+        }
+      } else {
+        var botmsg := PKV.GetMessage(bot, botidx);
+        var topmsg := PKV.GetMessage(top, topidx);
+        var newmsg := ValueMessage.Merge(topmsg, botmsg);
+        var encoded_newmsg := PKV.Message_to_bytestring(newmsg);
+        var kvweight := 4 + |topkey| as uint64 + 4 + |encoded_newmsg| as uint64;
+        if newmsg != IdentityMessage() {
+          var kvweight := 4 + |topkey| as uint64 + 4 + |encoded_newmsg| as uint64;
+          if kvweight < runningSlack {
+            dresult.AppendEncodedMessage(topkey, encoded_newmsg);
+            runningSlack := runningSlack - kvweight;
+          } else {
+            break;
+          }
+        } else {
+          var kvweight := 4 + |botkey| as uint64 + 4 + |PSA.psaElement(bot.messages, botidx)| as uint64;
+          runningSlack := runningSlack + kvweight;
+        }
+        topidx := topidx + 1;
+        botidx := botidx + 1;
+      }
+    }
+
+    while topidx < to
+      invariant from <= topidx <= to
+      invariant dresult.WF()
+      invariant dresult.keys.nstrings <= botidx + topidx - from
+      invariant runningSlack <= slack
+      invariant dresult.keys.nstrings <= botidx + topidx - from
+      invariant dresult.weight() <= PKV.WeightPkv(PKV.subPkv(bot, 0, botidx)) + slack - runningSlack
+      invariant fresh(dresult.Repr)
+      invariant 0 < |PSA.I(dresult.keys.toPsa())| && topidx < to ==>
+        PKV.Keyspace.lt(Seq.Last(PSA.I(dresult.keys.toPsa())), PSA.I(top.keys)[topidx])
+      invariant PKV.Keyspace.IsStrictlySorted(PSA.I(dresult.keys.toPsa()))
+    {
+      var topkey := PKV.GetKey(top, topidx);
+      var topmsg := PSA.psaElement(top.messages, topidx);
+      var kvweight := 4 + |topkey| as uint64 + 4 + |topmsg| as uint64;
+      assert topmsg == PSA.I(top.messages)[topidx];
+      if topidx + 1 < to {
+        PKV.Keyspace.IsStrictlySortedImpliesLt(PSA.I(top.keys), topidx as nat, topidx as nat + 1);
+      }
+      if PSA.psaCanAppend(dresult.keys.toPsa(), PSA.I(top.keys)[topidx]) {
+        PSA.psaAppendIAppend(dresult.keys.toPsa(), PSA.I(top.keys)[topidx]);
+        PKV.Keyspace.StrictlySortedAugment(PSA.I(dresult.keys.toPsa()), PSA.I(top.keys)[topidx]);
+      }
+      if kvweight < runningSlack {
+        dresult.AppendEncodedMessage(topkey, topmsg);
+        runningSlack := runningSlack - kvweight;
+        topidx := topidx + 1;
+      } else {
+        break;
+      }
+    }
+
+    while botidx < PKV.NumKVPairs(bot)
+      invariant botidx <= PKV.NumKVPairs(bot)
+      invariant dresult.WF()
+      invariant dresult.keys.nstrings <= botidx + topidx - from
+      invariant runningSlack <= slack
+      invariant dresult.keys.nstrings <= botidx + topidx - from
+      invariant dresult.weight() <= PKV.WeightPkv(PKV.subPkv(bot, 0, botidx)) + slack - runningSlack
+      invariant fresh(dresult.Repr)
+      invariant 0 < |PSA.I(dresult.keys.toPsa())| && botidx as nat < |PSA.I(bot.keys)| ==>
+        PKV.Keyspace.lt(Seq.Last(PSA.I(dresult.keys.toPsa())), PSA.I(bot.keys)[botidx])
+      invariant PKV.Keyspace.IsStrictlySorted(PSA.I(dresult.keys.toPsa()))
+    {
+      var botkey := PKV.GetKey(bot, botidx);
+      var botmsg := PSA.psaElement(bot.messages, botidx);
+      assert botmsg == PSA.I(bot.messages)[botidx];
+      if botidx as nat + 1 < |PSA.I(bot.keys)| {
+        PKV.Keyspace.IsStrictlySortedImpliesLt(PSA.I(bot.keys), botidx as nat, botidx as nat + 1);
+      }
+      PSA.psaAppendIAppend(dresult.keys.toPsa(), PSA.I(bot.keys)[botidx]);
+      PKV.Keyspace.StrictlySortedAugment(PSA.I(dresult.keys.toPsa()), PSA.I(bot.keys)[botidx]);
+      dresult.AppendEncodedMessage(botkey, botmsg);
+      // no change in slack
+      botidx := botidx + 1;
+    }
+
+    if topidx == to {
+      result := MergeCompleted(dresult.toPkv(), runningSlack);
+    } else {
+      result := SlackExhausted(dresult.toPkv(), topidx, runningSlack);
+    }
+  }
+
+  datatype MergeResult = MergeResult(top: PKV.Pkv, bots: seq<PKV.Pkv>, slack: uint64)
+  
+  method DoMergeToChildren(top: PKV.Pkv, pivotIdxs: seq<uint64>, bots: seq<PKV.Pkv>, slack: uint64) returns (result: MergeResult)
+    requires PKV.WF(top)
+    requires Uint64_Order.IsSorted(pivotIdxs)
+    requires 0 < |bots| == |pivotIdxs| < Uint64UpperBound()
+    requires Seq.Last(pivotIdxs) <= PKV.NumKVPairs(top)
+    requires forall i | 0 <= i < |bots| :: PKV.WF(bots[i])
+  {
+    var tmp: SingleMergeResult;
+    var runningSlack: uint64 := slack;
+    var results := new PKV.Pkv[|bots| as uint64];
+
+    Uint64_Order.IsSortedImpliesLte(pivotIdxs, 0, |pivotIdxs|-1);
+    tmp := MergeToOneChild(top, 0, pivotIdxs[0], bots[0], runningSlack);
+    results[0] := tmp.bot;
+    runningSlack := tmp.slack;
+    
+    var i: uint64 := 1;
+    while i < |bots| as uint64
+      invariant i <= |bots| as uint64
+      invariant tmp.SlackExhausted? ==> tmp.end < PKV.NumKVPairs(top)
+    {
+      Uint64_Order.IsSortedImpliesLte(pivotIdxs, i as int - 1, i as int);
+      Uint64_Order.IsSortedImpliesLte(pivotIdxs, i as int, |pivotIdxs|-1);
+      if tmp.MergeCompleted? {
+        tmp := MergeToOneChild(top, pivotIdxs[i-1], pivotIdxs[i], bots[i], runningSlack);
+        results[i] := tmp.bot;
+        runningSlack := tmp.slack;
+      } else {
+        // Once we exhaust our slack on one child, we just copy the
+        // remaining children
+        //
+        // XXX/FIXME/TODO[robj]: Do we want to copy the pkvs in this
+        // situation?  I suspect not.
+        results[i] := bots[i];
       }
       i := i + 1;
     }
-    return true;
+
+    if tmp.SlackExhausted? {
+      var leftover_top := PKV.SubPkv(top, tmp.end, PKV.NumKVPairs(top));
+      result := MergeResult(leftover_top, results[..], runningSlack);
+    } else {
+      result := MergeResult(PKV.EmptyPkv(), results[..], runningSlack);
+    }
+  }
+
+  method MergeToChildren(top: PKV.Pkv, pivots: seq<Key>, bots: seq<PKV.Pkv>, slack: uint64) returns (result: MergeResult)
+    requires PKV.WF(top)
+    requires PKV.Keyspace.IsStrictlySorted(PSA.I(top.keys))
+    requires PKV.Keyspace.IsStrictlySorted(pivots)
+    requires 0 < |bots| == |pivots| + 1 < Uint64UpperBound()
+    requires forall i | 0 <= i < |bots| :: PKV.WF(bots[i])
+  {
+    var pivotIdxs := PSA.PivotIndexes(top.keys, pivots);
+    forall i, j | 0 <= i <= j < |pivotIdxs|
+      ensures pivotIdxs[i] <= pivotIdxs[j]
+    {
+      if j < |pivotIdxs|-1 {
+        PKV.Keyspace.IndexOfFirstGteIsOrderPreserving(PSA.I(top.keys), pivots[i], pivots[j]);
+      } else {
+      }
+    }
+    assert Uint64_Order.IsSorted(pivotIdxs) by {
+      Uint64_Order.reveal_IsSorted();
+    }
+    result := DoMergeToChildren(top, pivotIdxs, bots, slack);
   }
 }
+
